Syntax.v
@@ -1,27 +1,42 @@
-Require Import SGA.Common SGA.TypedSyntax.
+Require Export SGA.Common SGA.Types SGA.ErrorReporting.
 
 Section Syntax.
-  Context {pos_t rule_name_t method_name_t var_t: Type}.
+  Context {pos_t rule_name_t fn_name_t var_t: Type}.
 
-  Inductive uaction {reg_t fn_t} :=
-  | UError
+  Inductive uaction {reg_t ufn_t} :=
+  | UError (err: error pos_t var_t fn_name_t)
   | UFail (tau: type)
   | UVar (var: var_t)
   | UConst {tau: type} (cst: type_denote tau)
-  | UConstString (s: string)
-  | UConstEnum (sig: enum_sig) (cst: string)
   | UAssign (v: var_t) (ex: uaction)
-  | USeq (r1 r2: uaction)
+  | USeq (a1 a2: uaction)
   | UBind (v: var_t) (ex: uaction) (body: uaction)
   | UIf (cond: uaction) (tbranch: uaction) (fbranch: uaction)
   | URead (port: Port) (idx: reg_t)
   | UWrite (port: Port) (idx: reg_t) (value: uaction)
-  | UCall (fn: fn_t) (arg1: uaction) (arg2: uaction)
-  | UCallModule {module_reg_t: Type} {module_fn_t: Type}
-                (fR: module_reg_t -> reg_t) (fSigma: module_fn_t -> fn_t)
-                (body: @uaction module_reg_t module_fn_t)
-  | UInternalCall (sig: @InternalSignature method_name_t var_t) (body: uaction) (args: list uaction)
-  | UAPos (p: pos_t) (e: uaction).
+  | UCall (fn: ufn_t) (arg1: uaction) (arg2: uaction)
+  | UInternalCall (sig: @InternalSignature fn_name_t var_t)
+                  (body: uaction) (args: list uaction)
+  | UAPos (p: pos_t) (e: uaction)
+  | USugar (s: usugar)
+  with usugar {reg_t ufn_t} :=
+  | USkip
+  | UProgn (aa: list uaction)
+  | UConstBits {sz} (bs: bits sz)
+  | UConstString (s: string)
+  | UConstEnum (sig: enum_sig) (cst: string)
+  | UStructInit (sig: struct_sig) (fields: list (string * uaction))
+  | USwitch (var: uaction)
+            (default: uaction)
+            (branches: list (uaction * uaction))
+  | UCallModule {module_reg_t: Type} {module_ufn_t: Type}
+                (fR: module_reg_t -> reg_t)
+                (fSigma: module_ufn_t -> ufn_t)
+                (sig: @InternalSignature fn_name_t var_t)
+                (body: @uaction module_reg_t module_ufn_t)
+                (args: list uaction).
+
+  Coercion USugar: usugar >-> uaction.
 
   Inductive uscheduler :=
   | UDone
@@ -30,5 +45,6 @@ Section Syntax.
   | USPos (p: pos_t) (s: uscheduler).
 End Syntax.
 
+Arguments usugar : clear implicits.
 Arguments uaction : clear implicits.
 Arguments uscheduler : clear implicits.
