Desugaring.v
@@ -1,0 +1,104 @@
+Require Import SGA.Common SGA.Environments SGA.Syntax SGA.TypedSyntax SGA.ErrorReporting SGA.SyntaxMacros SGA.Interop.
+Require Import Coq.Lists.List.
+Import ListNotations.
+
+Section Desugaring.
+  (* The desugaring phase can produce larger terms than its inputs, and so
+     cannot be intermingled with the typechecking phase without angering
+     Coq's termination checker. *)
+
+  Context {pos_t var_t fn_name_t reg_t ext_fn_t: Type}.
+
+  Notation usugar := (usugar pos_t var_t fn_name_t).
+  Notation uaction := (uaction pos_t var_t fn_name_t).
+
+  Import PrimUntyped.
+
+  Fixpoint desugar_UProgn {reg_t ufn_t} (aa: list (uaction reg_t ufn_t)) :=
+    match aa with
+    | [] => UConst (tau := bits_t 0) Ob
+    | [a] => a
+    | a :: aa => USeq a (desugar_UProgn aa)
+    end.
+
+  Fixpoint desugar_USwitch
+           (var: uaction reg_t ext_fn_t)
+           (default: uaction reg_t ext_fn_t)
+           (branches: list (uaction reg_t ext_fn_t *
+                            uaction reg_t ext_fn_t))
+    : uaction reg_t ext_fn_t :=
+    match branches with
+    | nil => default
+    | (val, action) :: branches =>
+      UIf (UBinOp UEq var val) action (desugar_USwitch var default branches)
+    end.
+
+  Definition map_int_fn_body {fn_name_t var_t action action': Type}
+             (f: action -> action') (fn: InternalFunction fn_name_t var_t action) :=
+    {| int_name := fn.(int_name);
+       int_argspec := fn.(int_argspec);
+       int_retType := fn.(int_retType);
+       int_body := f fn.(int_body) |}.
+
+  Fixpoint desugar_action' {reg_t' ext_fn_t'} (pos: pos_t)
+           (fR: reg_t' -> reg_t) (fSigma: ext_fn_t' -> ext_fn_t)
+           (a: uaction reg_t' ext_fn_t') {struct a}
+    : uaction reg_t ext_fn_t :=
+    let d a := desugar_action' pos fR fSigma a in
+    match a with
+    | UError err => UError err
+    | UFail tau => UFail tau
+    | UVar var => UVar var
+    | UConst cst => UConst cst
+    | UAssign v ex => UAssign v (d ex)
+    | USeq a1 a2 => USeq (d a1) (d a2)
+    | UBind v ex body => UBind v (d ex) (d body)
+    | UIf cond tbranch fbranch => UIf (d cond) (d tbranch) (d fbranch)
+    | URead port idx => URead port (fR idx)
+    | UWrite port idx value => UWrite port (fR idx) (d value)
+    | UUnOp fn arg => UUnOp fn (d arg)
+    | UBinOp fn arg1 arg2 => UBinOp fn (d arg1) (d arg2)
+    | UExternalCall fn arg => UExternalCall (fSigma fn) (d arg)
+    | UInternalCall fn args => UInternalCall (map_int_fn_body d fn) (List.map d args)
+    | UAPos p e => UAPos p (d e)
+    | USugar s => desugar pos fR fSigma s
+    end
+  with desugar {reg_t' ext_fn_t'}
+               (pos: pos_t)
+               (fR: reg_t' -> reg_t) (fSigma: ext_fn_t' -> ext_fn_t)
+               (s: usugar reg_t' ext_fn_t')
+       : uaction reg_t ext_fn_t :=
+         let d a := desugar_action' pos fR fSigma a in
+         match s with
+         | USkip =>
+           UConst (tau := bits_t 0) Ob
+         | UProgn aa =>
+           desugar_UProgn (List.map d aa)
+         | UConstBits bs =>
+           UConst (tau := bits_t _) bs
+         | UConstString s =>
+           UConst (tau := bits_t _) (bits_of_bytes s)
+         | UConstEnum sig name =>
+           match vect_index name sig.(enum_members) with
+           | Some idx => UConst (tau := enum_t sig) (vect_nth sig.(enum_bitpatterns) idx)
+           | None => UError {| epos := pos; emsg := UnboundEnumMember name sig;
+                              esource := ErrSrc s |}
+           end
+         | UStructInit sig fields =>
+           let uinit := UUnOp (UConv (UUnpack (struct_t sig))) in
+           let usubst f := UBinOp (UStruct2 (USubstField f)) in
+           List.fold_left (fun acc '(f, a) => (usubst f) acc (d a))
+                          fields (uinit (UConst (tau := bits_t _) (Bits.zero (struct_sz sig))))
+         | USwitch var default branches =>
+           let branches := List.map (fun '(cond, body) => (d cond, d body)) branches in
+           desugar_USwitch (d var) (d default) branches
+         | UCallModule fR' fSigma' fn args =>
+           let df body := desugar_action' pos (fun r => fR (fR' r)) (fun fn => fSigma (fSigma' fn)) body in
+           let args := List.map d args in
+           UInternalCall (map_int_fn_body df fn) args
+         end.
+
+  Definition desugar_action (pos: pos_t) (a: uaction reg_t ext_fn_t)
+    : uaction reg_t ext_fn_t :=
+    desugar_action' pos (fun r => r) (fun fn => fn) a.
+End Desugaring.
