ErrorReporting.v
@@ -1,0 +1,52 @@
+Require Import SGA.Common SGA.Types.
+
+Section TypeErrors.
+  Context {pos_t var_t fn_name_t: Type}.
+
+  Inductive basic_error_message :=
+  | UnboundField (f: string) (sig: struct_sig)
+  | TypeMismatch (actual: type) (expected: type)
+  | KindMismatch (actual: type_kind) (expected: type_kind).
+
+  Inductive error_message :=
+  | ExplicitErrorInAst
+  | SugaredConstructorInAst
+  | UnboundVariable (var: var_t)
+  | UnboundEnumMember (f: string) (sig: enum_sig)
+  | IncorrectRuleType (tau: type)
+  | BasicError (msg: basic_error_message)
+  | TooManyArguments (fn_name: fn_name_t) (nexpected: nat) (nextra: nat)
+  | TooFewArguments (fn_name: fn_name_t) (nexpected: nat) (nmissing: nat).
+
+  (* FIXME add ability to report error on meta arguments *)
+  (* FIXME and use this to fix the location of unbound field errors *)
+  Inductive fn_tc_error_loc := Arg1 | Arg2.
+  Definition fn_tc_error : Type := fn_tc_error_loc * basic_error_message.
+
+  Definition assert_bits_t arg (tau: type) : result nat fn_tc_error :=
+    match tau with
+    | bits_t sz => Success sz
+    | enum_t _ | struct_t _ => Failure (arg, KindMismatch (kind_of_type tau) kind_bits)
+    end.
+
+  Definition assert_struct_t arg (tau: type) : result struct_sig fn_tc_error :=
+    match tau with
+    | struct_t sg => Success sg
+    | bits_t _ | enum_t _ => Failure (arg, KindMismatch (kind_of_type tau) (kind_struct None))
+    end.
+
+  (* Error sources live in prop, because they are only useful in interactive
+     mode: LV only cares about positions. *)
+  Inductive ErrorSource : Prop :=
+  | ErrSrc {T: Type} (t: T).
+
+  Record error :=
+    { epos: pos_t;
+      emsg: error_message;
+      esource: ErrorSource }.
+End TypeErrors.
+
+Arguments basic_error_message : clear implicits.
+Arguments fn_tc_error : clear implicits.
+Arguments error_message : clear implicits.
+Arguments error : clear implicits.
