Extraction.v
@@ -29,7 +29,7 @@ Extraction "SGA.ml"
            IndexUtils.List_nth
            Environments.ContextEnv Environments.to_list
            Vect.vect_to_list Vect.vect_of_list Vect.Bits.to_nat Vect.index_to_nat Vect.vect_zip
-           Syntax.uscheduler SyntaxMacros.USkip SyntaxMacros.UConstBits SyntaxMacros.USwitch SyntaxMacros.UStructInit
+           Syntax.uscheduler
            TypeInference.type_action TypeInference.type_rule TypeInference.type_scheduler
            SyntaxTools.action_mentions_var SyntaxTools.member_mentions_shadowed_binding
            Circuits.compile_scheduler
