TypedSyntax.v
@@ -1,9 +1,6 @@
 Require Import Coq.Lists.List.
 Require Export SGA.Common SGA.Environments SGA.Types.
 
-Inductive Port :=
-  P0 | P1.
-
 Section TypedSyntax.
   Context {name_t var_t reg_t fn_t: Type}.
   Context {R: reg_t -> type}
